some cleanup, and begin making max_cores a projection from the core state

veric/extension.v
@@ -50,9 +50,9 @@ Module Extension. Section Extension.
 
  Record Sig := Make {
  (** Generalized projection of genv, core [i] from state [s] *)
-  threads_max: nat;
+  proj_max_cores: xT -> nat;
   proj_core: forall i:nat, xT -> option (cT i); 
-  proj_threads_max: forall i s, i >= threads_max -> proj_core i s = None;
+  proj_core_proj_max: forall i s, i >= proj_max_cores s -> proj_core i s = None;
   active : xT -> nat; (** The active (i.e., currently scheduled) core *)
   active_proj_core : forall s, exists c, proj_core (active s) s = Some c;
   proj_zint: xT -> Zint; (** Type [xT] embeds [Zint]. *)
@@ -109,7 +109,6 @@ Section SafeExtension.
 
  Import Extension.
 
- (** a global invariant characterizing "safe" extensions *)
  Definition all_safe (E: Sig gT cT dT Zint esem csem csig esig handled)
   (n: nat) (z: Z) (w: xT) (m: M) :=
      forall i c, proj_core E i w = Some c -> 
@@ -163,116 +162,116 @@ Notation at_external_not_handled := E.(Extension.at_external_not_handled).
 Notation ext_upd_at_external := E.(Extension.ext_upd_at_external).
 
 Inductive safety_invariant: Type := SafetyInvariant: forall 
-  (** Coresteps preserve the all-safety invariant. *)
-  (core_pres: forall n z (s: xT) c m s' c' m', 
-    ALL_SAFE (S n) (s \o z) s m -> 
-    PROJ_CORE (ACTIVE s) s = Some c -> 
-    corestep (csem (ACTIVE s)) (genv_map (ACTIVE s)) c m c' m' -> 
-    corestep esem ge s m s' m' -> 
-    ALL_SAFE n (s' \o z) s' m')
+ (** Coresteps preserve the all-safety invariant. *)
+ (core_pres: forall n z (s: xT) c m s' c' m', 
+   ALL_SAFE (S n) (s \o z) s m -> 
+   PROJ_CORE (ACTIVE s) s = Some c -> 
+   corestep (csem (ACTIVE s)) (genv_map (ACTIVE s)) c m c' m' -> 
+   corestep esem ge s m s' m' -> 
+   ALL_SAFE n (s' \o z) s' m')
 
-  (** Corestates satisfying the invariant can corestep. *)
-  (core_prog: forall n z s m (c: cT (ACTIVE s)),
-    ALL_SAFE (S n) z s m -> 
-    PROJ_CORE (ACTIVE s) s = Some c -> 
-    runnable (csem (ACTIVE s)) c=true -> 
-    exists c', exists s', exists m', 
-      corestep (csem (ACTIVE s)) (genv_map (ACTIVE s)) c m c' m' /\ 
-      corestep esem ge s m s' m' /\
-      PROJ_CORE (ACTIVE s) s' = Some c')
+ (** Corestates satisfying the invariant can corestep. *)
+ (core_prog: forall n z s m (c: cT (ACTIVE s)),
+   ALL_SAFE (S n) z s m -> 
+   PROJ_CORE (ACTIVE s) s = Some c -> 
+   runnable (csem (ACTIVE s)) c=true -> 
+   exists c', exists s', exists m', 
+    corestep (csem (ACTIVE s)) (genv_map (ACTIVE s)) c m c' m' /\ 
+    corestep esem ge s m s' m' /\
+    PROJ_CORE (ACTIVE s) s' = Some c')
 
-  (** "Handled" steps respect function specifications. *)
-  (handled_pres: forall s z m (c: cT (ACTIVE s)) s' m' 
-        (c': cT (ACTIVE s)) ef sig args P Q x, 
-    let i := ACTIVE s in PROJ_CORE i s = Some c -> 
-    at_external (csem i) c = Some (ef, sig, args) -> 
-    ListSet.set_mem extfunct_eqdec ef handled = true -> 
-    spec_of ef csig = (P, Q) -> 
-    P x (sig_args sig) args (s \o z) m -> 
-    corestep esem ge s m s' m' -> 
-    PROJ_CORE i s' = Some c' -> 
-      ((at_external (csem i) c' = Some (ef, sig, args) /\ 
-        P x (sig_args sig) args (s' \o z) m' /\
-        (forall j, ACTIVE s' = j -> i <> j)) \/
-      (exists ret, after_external (csem i) ret c = Some c' /\ 
-        Q x (sig_res sig) ret (s' \o z) m')))
+ (** "Handled" steps respect function specifications. *)
+ (handled_pres: forall s z m (c: cT (ACTIVE s)) s' m' 
+     (c': cT (ACTIVE s)) ef sig args P Q x, 
+  let i := ACTIVE s in PROJ_CORE i s = Some c -> 
+   at_external (csem i) c = Some (ef, sig, args) -> 
+   ListSet.set_mem extfunct_eqdec ef handled = true -> 
+   spec_of ef csig = (P, Q) -> 
+   P x (sig_args sig) args (s \o z) m -> 
+   corestep esem ge s m s' m' -> 
+   PROJ_CORE i s' = Some c' -> 
+    ((at_external (csem i) c' = Some (ef, sig, args) /\ 
+      P x (sig_args sig) args (s' \o z) m' /\
+      (forall j, ACTIVE s' = j -> i <> j)) \/
+    (exists ret, after_external (csem i) ret c = Some c' /\ 
+      Q x (sig_res sig) ret (s' \o z) m')))
 
-  (** "Handled" states satisfying the invariant can step or are safely halted;
-     core states that remain "at_external" over handled steps are unchanged. *)
-  (handled_prog: forall n (z: Zext) (s: xT) m c,
-    ALL_SAFE (S n) (s \o z) s m -> 
-    PROJ_CORE (ACTIVE s) s = Some c -> 
-    runnable (csem (ACTIVE s)) c=false -> 
-    at_external esem s = None -> 
-    (exists s', exists m', corestep esem ge s m s' m' /\ 
-      forall i c, PROJ_CORE i s = Some c -> 
-        exists c', PROJ_CORE i s' = Some c' /\
-          (forall ef args ef' args', 
-            at_external (csem i) c = Some (ef, args) -> 
-            at_external (csem i) c' = Some (ef', args') -> c=c')) \/
-    (exists rv, safely_halted esem s = Some rv))
+ (** "Handled" states satisfying the invariant can step or are safely halted;
+    core states that remain "at_external" over handled steps are unchanged. *)
+ (handled_prog: forall n (z: Zext) (s: xT) m c,
+   ALL_SAFE (S n) (s \o z) s m -> 
+   PROJ_CORE (ACTIVE s) s = Some c -> 
+   runnable (csem (ACTIVE s)) c=false -> 
+   at_external esem s = None -> 
+   (exists s', exists m', corestep esem ge s m s' m' /\ 
+     forall i c, PROJ_CORE i s = Some c -> 
+       exists c', PROJ_CORE i s' = Some c' /\
+        (forall ef args ef' args', 
+          at_external (csem i) c = Some (ef, args) -> 
+          at_external (csem i) c' = Some (ef', args') -> c=c')) \/
+   (exists rv, safely_halted esem s = Some rv))
 
-  (** Safely halted threads remain halted. *)
-  (safely_halted_halted: forall s m s' m' i c rv,
-    PROJ_CORE i s = Some c -> 
-    safely_halted (csem i) c = Some rv -> 
-    corestep esem ge s m s' m' -> PROJ_CORE i s' = Some c)
+ (** Safely halted threads remain halted. *)
+ (safely_halted_halted: forall s m s' m' i c rv,
+   PROJ_CORE i s = Some c -> 
+   safely_halted (csem i) c = Some rv -> 
+   corestep esem ge s m s' m' -> PROJ_CORE i s' = Some c)
 
-  (** Safety of other threads is preserved when handling one step of blocked
-     thread [i]. *)
-  (handled_rest: forall s m s' m' c,
-    PROJ_CORE (ACTIVE s) s = Some c -> 
-    ((exists ef, exists sig, exists args, 
-        at_external (csem (ACTIVE s)) c = Some (ef, sig, args)) \/ 
-      exists rv, safely_halted (csem (ACTIVE s)) c = Some rv) -> 
-    at_external esem s = None -> 
-    corestep esem ge s m s' m' -> 
-    (forall j c0, ACTIVE s <> j ->  
-      (PROJ_CORE j s' = Some c0 -> PROJ_CORE j s = Some c0) /\
-      (forall n z z', PROJ_CORE j s = Some c0 -> 
-        safeN (csem j) csig (genv_map j) (S n) (s \o z) c0 m -> 
-        safeN (csem j) csig (genv_map j) n (s' \o z') c0 m')))
+ (** Safety of other threads is preserved when handling one step of blocked
+    thread [i]. *)
+ (handled_rest: forall s m s' m' c,
+   PROJ_CORE (ACTIVE s) s = Some c -> 
+   ((exists ef, exists sig, exists args, 
+      at_external (csem (ACTIVE s)) c = Some (ef, sig, args)) \/ 
+     exists rv, safely_halted (csem (ACTIVE s)) c = Some rv) -> 
+   at_external esem s = None -> 
+   corestep esem ge s m s' m' -> 
+   (forall j c0, ACTIVE s <> j ->  
+    (PROJ_CORE j s' = Some c0 -> PROJ_CORE j s = Some c0) /\
+    (forall n z z', PROJ_CORE j s = Some c0 -> 
+      safeN (csem j) csig (genv_map j) (S n) (s \o z) c0 m -> 
+      safeN (csem j) csig (genv_map j) n (s' \o z') c0 m')))
 
-  (** If the extended machine is at external, then the active thread is at
-     external (an extension only implements external functions, it doesn't
-     introduce them). *)
-  (at_extern_call: forall s ef sig args,
-    at_external esem s = Some (ef, sig, args) -> 
-    exists c, PROJ_CORE (ACTIVE s) s = Some c /\
-      at_external (csem (ACTIVE s)) c = Some (ef, sig, args))
+ (** If the extended machine is at external, then the active thread is at
+    external (an extension only implements external functions, it doesn't
+    introduce them). *)
+ (at_extern_call: forall s ef sig args,
+   at_external esem s = Some (ef, sig, args) -> 
+   exists c, PROJ_CORE (ACTIVE s) s = Some c /\
+    at_external (csem (ACTIVE s)) c = Some (ef, sig, args))
 
-  (** Inject the results of an external call into the extended machine state. *)
-  (at_extern_ret: forall z s (c: cT (ACTIVE s)) m z' m' tys args ty ret c' ef sig x 
-      (P: ext_spec_type esig ef -> list typ -> list val -> Zext -> M -> Prop) 
-      (Q: ext_spec_type esig ef -> option typ -> option val -> Zext -> M -> Prop),
-    PROJ_CORE (ACTIVE s) s = Some c -> 
-    at_external esem s = Some (ef, sig, args) -> 
-    spec_of ef esig = (P, Q) -> 
-    P x tys args (s \o z) m -> Q x ty ret z' m' -> 
-    after_external (csem (ACTIVE s)) ret c = Some c' -> 
-    exists s': xT, 
-      z' = s' \o z' /\
-      after_external esem ret s = Some s' /\ 
-      PROJ_CORE (ACTIVE s) s' = Some c')
+ (** Inject the results of an external call into the extended machine state. *)
+ (at_extern_ret: forall z s (c: cT (ACTIVE s)) m z' m' tys args ty ret c' ef sig x 
+    (P: ext_spec_type esig ef -> list typ -> list val -> Zext -> M -> Prop) 
+    (Q: ext_spec_type esig ef -> option typ -> option val -> Zext -> M -> Prop),
+   PROJ_CORE (ACTIVE s) s = Some c -> 
+   at_external esem s = Some (ef, sig, args) -> 
+   spec_of ef esig = (P, Q) -> 
+   P x tys args (s \o z) m -> Q x ty ret z' m' -> 
+   after_external (csem (ACTIVE s)) ret c = Some c' -> 
+   exists s': xT, 
+    z' = s' \o z' /\
+    after_external esem ret s = Some s' /\ 
+    PROJ_CORE (ACTIVE s) s' = Some c')
 
-  (** Safety of other threads is preserved when returning from an external 
-     function call. *)
-  (at_extern_rest: forall z s (c: cT (ACTIVE s)) m z' s' m' tys args ty ret c' ef x sig
-      (P: ext_spec_type esig ef -> list typ -> list val -> Zext -> M -> Prop) 
-      (Q: ext_spec_type esig ef -> option typ -> option val -> Zext -> M -> Prop),
-    PROJ_CORE (ACTIVE s) s = Some c -> 
-    at_external esem s = Some (ef, sig, args) -> 
-    spec_of ef esig = (P, Q) -> 
-    P x tys args (s \o z) m -> Q x ty ret z' m' -> 
-    after_external (csem (ACTIVE s)) ret c = Some c' -> 
-    after_external esem ret s = Some s' -> 
-    PROJ_CORE (ACTIVE s) s' = Some c' ->  
-    (forall j (CS0: CoreSemantics (gT j) (cT j) M (dT j)) c0, ACTIVE s <> j -> 
-      (PROJ_CORE j s' = Some c0 -> PROJ_CORE j s = Some c0) /\
-      (forall ge n, PROJ_CORE j s = Some c0 -> 
-        safeN CS0 csig ge (S n) (s \o z) c0 m -> 
-        safeN CS0 csig ge n (s' \o z') c0 m'))),
-  safety_invariant.
+ (** Safety of other threads is preserved when returning from an external 
+    function call. *)
+ (at_extern_rest: forall z s (c: cT (ACTIVE s)) m z' s' m' tys args ty ret c' ef x sig
+    (P: ext_spec_type esig ef -> list typ -> list val -> Zext -> M -> Prop) 
+    (Q: ext_spec_type esig ef -> option typ -> option val -> Zext -> M -> Prop),
+   PROJ_CORE (ACTIVE s) s = Some c -> 
+   at_external esem s = Some (ef, sig, args) -> 
+   spec_of ef esig = (P, Q) -> 
+   P x tys args (s \o z) m -> Q x ty ret z' m' -> 
+   after_external (csem (ACTIVE s)) ret c = Some c' -> 
+   after_external esem ret s = Some s' -> 
+   PROJ_CORE (ACTIVE s) s' = Some c' ->  
+   (forall j (CS0: CoreSemantics (gT j) (cT j) M (dT j)) c0, ACTIVE s <> j -> 
+    (PROJ_CORE j s' = Some c0 -> PROJ_CORE j s = Some c0) /\
+    (forall ge n, PROJ_CORE j s = Some c0 -> 
+      safeN CS0 csig ge (S n) (s \o z) c0 m -> 
+      safeN CS0 csig ge n (s' \o z') c0 m'))),
+ safety_invariant.
 
 End SafetyInvariant. End SafetyInvariant.
 
@@ -304,3 +303,104 @@ Import SafetyInvariant.
 Record Sig := Make {_: safety_invariant ge genv_map E -> safe_extension ge genv_map E}.
 
 End EXTENSION_SAFETY. End EXTENSION_SAFETY.
+
+(** Some administrative requirements on the interactions between extensions and
+   inner cores. Perhaps some of these conditions could be merged with those for
+   "safe" extensions. *)
+
+Section CoreCompatible.
+ Variables
+  (G: Type) (** global environments *)
+  (D: Type) (** initialization data *)
+  (xT: Type) (** corestates of extended semantics *)
+  (gT: nat -> Type) (** global environments of the core semantics *)
+  (cT: nat -> Type) (** corestates of core semantics *)
+  (M: Type) (** memories *)
+  (dT: nat -> Type) (** initialization data *)
+  (Z: Type) (** external states *)
+  (Zint: Type) (** portion of Z implemented by extension *)
+  (Zext: Type) (** portion of Z external to extension *)
+
+  (esem: CoreSemantics G xT M D) (** extended semantics *)
+  (csem: forall i:nat, CoreSemantics (gT i) (cT i) M (dT i)) (** a set of core semantics *)
+
+  (csig: ef_ext_spec M Z) (** client signature *)
+  (esig: ef_ext_spec M Zext) (** extension signature *)
+  (handled: list AST.external_function). (** functions handled by this extension *)
+
+Variables (ge: G) (genv_map : forall i:nat, gT i).
+Variable E: Extension.Sig gT cT dT Zint esem csem csig esig handled.
+
+Import Extension.
+
+Inductive core_compatible: Type := CoreCompatible: forall
+ (** When the active thread is runnable, a step in the extended semantics can be
+    tracked back to a corestep of the active thread. *)
+ (runnable_corestep: forall s m s' m' c,
+   runnable (csem (active E s)) c=true -> 
+   proj_core E (active E s) s = Some c -> 
+   corestep esem ge s m s' m' -> 
+   exists c', corestep (csem (active E s)) (genv_map (active E s)) c m c' m' /\ 
+    proj_core E (active E s) s' = Some c') 
+
+ (** After a corestep of the active inner core, the active thread's new
+    corestate is appropriately injected into the extended state. *)
+ (corestep_pres: forall s (c: cT (active E s)) m c' s' m',
+   proj_core E (active E s) s = Some c -> 
+   corestep (csem (active E s)) (genv_map (active E s)) c m c' m' -> 
+   corestep esem ge s m s' m' -> 
+   active E s = active E s' /\ 
+   proj_core E (active E s) s' = Some c')
+
+ (** A corestep of the currently active core forces a corestep of the extended
+    semantics*)
+ (corestep_prog: forall s (c: cT (active E s)) m c' m',
+   proj_core E (active E s) s = Some c -> 
+   corestep (csem (active E s)) (genv_map (active E s)) c m c' m' -> 
+   exists s', corestep esem ge s m s' m')
+
+ (** Other cores remain unchanged after coresteps of the active core. *)
+ (corestep_others_forward: forall s s' (c: cT (active E s')) m c' m',
+   active E s=active E s' -> 
+   proj_core E (active E s') s' = Some c' -> 
+   corestep (csem (active E s')) (genv_map (active E s')) c m c' m' -> 
+   corestep esem ge s m s' m' -> 
+   forall j, (active E s)<>j -> proj_core E j s = proj_core E j s')
+ (corestep_others_backward: forall s c m s' c' m' n,
+   proj_core E (active E s) s = Some c -> 
+   corestepN (csem (active E s)) (genv_map (active E s)) n c m c' m' -> 
+   corestepN esem ge n s m s' m' -> 
+   forall j, (active E s)<>j -> proj_core E j s = proj_core E j s')
+
+ (** The active core id doesn't change along active coresteps. *)
+ (after_ext_pres: forall s (c: cT (active E s)) c' s' retv,
+   proj_core E (active E s) s = Some c -> 
+   after_external (csem (active E s)) retv c = Some c' -> 
+   after_external esem retv s = Some s' -> 
+   active E s=active E s')
+
+ (** Extension states can be updated to match after_external on the active
+    core. *)
+ (after_ext_prog: forall s (c: cT (active E s)) c' retv,
+   proj_core E (active E s) s = Some c -> 
+   after_external (csem (active E s)) retv c = Some c' -> 
+   exists s', after_external esem retv s = Some s' /\
+    proj_core E (active E s) s' = Some c')
+
+ (** after_external on extension cores leaves all but the active corestate
+    unchanged. *)
+ (after_ext_others: forall s s' retv,
+   after_external esem retv s = Some s' -> 
+   forall j, (active E s)<>j -> 
+    proj_core E j s = proj_core E j s')
+
+ (** Hypothesis repeated from extension signature to get around a bug in
+ [Program]. *)
+ (at_extern_call: forall s ef sig args,
+   at_external esem s = Some (ef, sig, args) -> 
+   exists c, proj_core E (active E s) s = Some c /\
+    at_external (csem (active E s)) c = Some (ef, sig, args)),
+ core_compatible.
+
+End CoreCompatible.
+
